providers/evercrypt/EverCrypt.AEAD.fsti
@@ -1,0 +1,68 @@
+module EverCrypt.AEAD
+
+module S = FStar.Seq
+module G = FStar.Ghost
+
+module HS = FStar.HyperStack
+module ST = FStar.HyperStack.ST
+module MB = LowStar.Monotonic.Buffer
+module B = LowStar.Buffer
+
+open FStar.HyperStack.ST
+open FStar.Integers
+
+open Spec.AEAD
+
+noextract
+let bytes = Seq.seq UInt8.t
+
+let frozen_preorder (s: bytes): MB.srel UInt8.t = fun (s1 s2: bytes) ->
+  S.equal s1 s ==> S.equal s2 s
+
+noeq
+type expanded_key (a: alg) =
+| EK:
+    kv:G.erased (kv a) -> ek:(
+    let s = expand (G.reveal kv) in
+    let p = frozen_preorder s in
+    ek:MB.mbuffer UInt8.t p p { MB.witnessed ek (S.equal s) }) ->
+    expanded_key a
+
+val expand_in:
+  #a:alg ->
+  r:HS.rid ->
+  k:B.buffer UInt8.t { B.length k = key_length a } ->
+  ST (expanded_key a)
+    (requires fun h0 ->
+      B.live h0 k)
+    (ensures fun h0 ek h1 ->
+      let l = B.loc_buffer (EK?.ek ek) in
+      Hash.fresh_loc l h0 h1 /\
+      B.(modifies loc_none h0 h1) /\
+      B.(loc_includes (loc_region_only true r) l) /\
+      S.equal (G.reveal (EK?.kv ek)) (B.as_seq h0 k))
+
+let iv_p a = iv:B.buffer UInt8.t { B.length iv = iv_length a }
+let ad_p a = ad:B.buffer UInt8.t { B.length ad <= max_length a }
+let plain_p a = p:B.buffer UInt8.t { B.length p <= max_length a }
+
+val encrypt:
+  #a:alg ->
+  ek:expanded_key a ->
+  iv:iv_p a ->
+  ad:ad_p a ->
+  ad_len: UInt32.t { v ad_len = B.length ad } ->
+  plain: plain_p a ->
+  plain_len: UInt32.t { v plain_len = B.length plain } ->
+  dst: B.buffer UInt8.t { B.length dst = B.length plain + tag_length a } ->
+  Stack unit
+    (requires fun h0 ->
+      B.live h0 (EK?.ek ek) /\
+      B.live h0 iv /\
+      B.live h0 ad /\
+      B.live h0 plain /\
+      B.live h0 dst)
+    (ensures fun h0 _ h1 ->
+      B.(modifies (loc_buffer dst) h0 h1) /\
+      S.equal (B.as_seq h1 dst)
+        (encrypt (G.reveal (EK?.kv ek)) (B.as_seq h0 iv) (B.as_seq h0 ad) (B.as_seq h0 plain)))
